\newtheorem*{SUMTOARA}{Proposition~\ref{prop:sum_to_ara}}

We prove proposition \ref{prop:sum_to_ara}.

\begin{SUMTOARA}
  For each \langsum expression $e$ over schema $\Sch$ such that $\Sch(e)=(\alpha,\beta)$ with $\alpha\neq 1\neq\beta$, there exists an $\mathsf{RA}_{K}^+$  expression $\Phi(e)$ over relational schema $\text{Rel}(\Sch)$ such that $\text{Rel}(\Sch)(\Phi(e))=\{\row_\alpha,\row_\beta\}$ and 
	such that for any instance $\I$ over~$\Sch$,
	$$
	\sem{e}{\I}_{i,j}=\ssem{\Phi(e)}{\text{Rel}(\I)}(t)
	$$
	for tuple $t(\mathrm{row}_\alpha)=i$ and $t(\mathrm{col}_\beta)=j$. Similarly for when $e$ has schema $\Sch(e)=(\alpha,1)$, $\Sch(e)=(1,\beta)$ or $\Sch(e)=(1,1)$, then $\Phi(e)$ has schema $\text{Rel}(\Sch)(\Phi(e))=\{\mathrm{row}_\alpha\}$,
	$\text{Rel}(\Sch)(\Phi(e))=\{\mathrm{col}_\alpha\}$, or
	$\text{Rel}(\Sch)(\Phi(e))=\{\}$, respectively.
\end{SUMTOARA}

\textit{Proof}. We start from a matrix schema $\Sch=(\Mnam,\size)$, where $\Mnam\subset \Mvar$ is a finite set of matrix variables, 
and $\size: \Mvar \mapsto \DD\times \DD$ is a function that maps each matrix variable to a pair of size symbols. 
On the relational side we have for each size symbol $\alpha\in\DD\setminus\{1\}$, attributes $\alpha$, $\row_\alpha$, 
and $\col_\alpha$ in $\att$. For each $V\in\Mnam$ and $\alpha \in \DD$ we denote
by $R_V$ and $R_\alpha$ its corresponding relation name, respectively. Then, given $\Sch$ we define the relational 
schema $\text{Rel}(\Sch)$ such that $\fdom(\text{Rel}(\Sch)) =  \{R_\alpha \mid \alpha\in\DD\} \cup \{R_V \mid V \in \Mnam\}$ 
where $\text{Rel}(\Sch)(R_\alpha) = \{\alpha\}$ and:
\[
\text{Rel}(\Sch)(R_V) = \begin{cases}
\lbrace\row_\alpha,\col_\beta \rbrace & \text{ if $ \size(V)=(\alpha,\beta)$} \\
\lbrace\row_\alpha \rbrace & \text{ if $ \size(V)=(\alpha,1)$} \\
\lbrace\col_\beta \rbrace  &
\text{ if $ \size(V)=(1,\beta)$} \\
\lbrace\rbrace & \text{ if $\size(V)=(1,1)$}.
\end{cases}
\]
Next, for a matrix instance $\I = (\dom,\conc)$ over $\Sch$,
let $V\in\Mnam$ with $\size(V)=(\alpha,\beta)$ and let $\conc(V)$ be its corresponding $K$-matrix of dimension $\dom(\alpha)\times \dom(\beta)$.
The $K$-instance in ARA according to $\I$ is $\text{Rel}(\I)$ with data domain $\ddom = \mathbb{N} \setminus \{0\}$. For each $V\in\Mnam$ we define 
$R_V^{\text{Rel}(\I)}(t):=\conc(V)_{ij}$ whenever $t(\row_\alpha) = i \leq \dom(\alpha)$ and $t(\col_\beta) = j \leq \dom(\beta)$, and $\kzero$ otherwise. 
Also, for each $\alpha \in \DD$ we define $R_\alpha^{\text{Rel}(\I)}(t):=\kone$ whenever $t(\alpha) \leq \dom(\alpha)$, and $\kzero$ otherwise.
If $\size(V)=(\alpha,1)$ then $R_V^{\text{Rel}(\I)}(t):=\conc(V)_{i1}$ whenever $t(\row_\alpha) = i \leq \dom(\alpha)$ and $\kzero$ otherwise.
Similarly, if $\size(V)=(1,\beta)$ then $R_V^{\text{Rel}(\I)}(t):=\conc(V)_{1j}$ whenever $t(\col_\beta) = j \leq \dom(\beta)$ and $\kzero$ otherwise.
If $\size(V)=(1,1)$ then $R_V^{\text{Rel}(\I)}(t):=\conc(V)_{11}$ only when $t(1) = \kone$ and $\kzero$ otherwise.

The proof is by induction. Let $e$ be a \langsum expression such that $\Sch (e)=(\alpha, \beta)$.
\begin{itemize}
  \item If $e=V$ then $\Phi (e):=R_V^{\text{Rel}(\I)}$.

  \item If $e=e_1^T$ with $\Sch (e_1)=(\alpha, \beta)$ then \[
\Phi(e) :=
\begin{cases}
\rho_{\mathrm{row}_\alpha \to \mathrm{col}_\alpha,\mathrm{col}_\beta \to \mathrm{row}_\beta}\bigl(\Phi(e_1)\bigr) & \text{if } \alpha \neq 1 \neq \beta; \cr
\rho_{\mathrm{row}_\alpha \to \mathrm{col}_\alpha}\bigl(\Phi(e_1)\bigr) & \text{if } \alpha \neq 1 = \beta; \cr
\rho_{\mathrm{col}_\beta \to \mathrm{row}_\beta}\bigl(\Phi(e_1)\bigr) & \text{if } \alpha = 1 \neq \beta; \cr
\Phi(e_1) & \text{if } \alpha = 1 = \beta,
\end{cases}
\]

  \item If $e=e_1+e_2$ with $\Sch (e_1)=\Sch (e_2)=(\alpha, \beta)$ then $\Phi (e):=\Phi (e_1)\cup \Phi (e_2)$.

  \item If $e=f(e_1,\ldots, e_k)$ with $\Sch(e_i)=(1,1)$ for all $i\in[1,k]$, with $f=\kprod$, then $\Phi(e):=\Phi(e_1)\Join \ldots \Join\Phi(e_k)$.

  \item If $e=e_1\cdot e_2$ with $\Sch (e_1)=(\alpha, \gamma)$ and $\Sch (e_2)=(\gamma, \beta)$, we have two cases. If $\gamma = 1$ then $\Phi (e):=\Phi (e_1)\Join \Phi (e_2)$.
If $\gamma\neq 1$ then
$$
\Phi (e) := \pi_{\lbrace \row_{\alpha},\row_{\beta} \rbrace}\left( \sigma_{\lbrace \col_\gamma, \row_\gamma \rbrace} \left( \Phi (e_1)\Join \Phi (e_2) \right) \right)
$$

%   \item If $e=\ssum V. e_1$ where $\Sch(e_1)=(\alpha,\beta)$ and $\Sch(V)=(\gamma,1)$. Then we can just do $\pi_{\text{Rel}(\Sch)(R_V)}\left( \Phi (e_1) \right)$.
% Note that when the $\row_\gamma$ attribute in $\Phi (e_1)$ is instantiated with with tuple $t$ such that $t(\row_\alpha)=i$, $t(\col_\beta)=j$ and $t(\row_\gamma)=k$,
% then the expression evaluates to $e_1(\I [V\leftarrow e_{k}^{\dom(\gamma)}])_{ij}$. 
% Hence, by projecting in attributes $\lbrace \row_\alpha, \col_\beta\rbrace$ we range over all $k$ and sum up all $K$-values for each entry.
  \item If $e=\ssum V. e_1$ where $\Sch(e_1)=(\alpha,\beta)$ and $\Sch(V)=(\gamma,1)$. Then we do 
  $$
  \pi_{\lbrace \row_{\alpha}, \col_{\beta} \rbrace}\left( \Phi (e_1)\left[ R_{V}^{\text{Rel}(\I)}\leftarrow R_{\mathsf{Id}}^{\gamma} \right] \right).
  $$
  Here $R_{\mathsf{Id}}^{\gamma}$ is the binary relation encoding the identity of size $\gamma\times\gamma$ and
  is defined as 
  $$
  R_{\mathsf{Id}}^{\gamma}:= \sigma_{\lbrace \row_{\gamma},\col_{\gamma} \rbrace }\left( \rho_{\gamma\rightarrow\row_\gamma}\left( R_\gamma^{\text{Rel}(\I)} \right) \Join \rho_{\gamma\rightarrow\col_\gamma}\left( R_\gamma^{\text{Rel}(\I)} \right)\right)
  $$
  Note that when $\Phi (e_1)\left[ R_{V}\leftarrow R_{\mathsf{Id}}^{\gamma} \right]$ is instantiated with with tuple $t$ such that $t(\row_\alpha)=i$, $t(\col_\beta)=j$, 
  $t(\row_\gamma)=k$ and $t(\col_\gamma)=k$ (other values of are zero),
  then the expression evaluates to $e_1(\I [V\leftarrow e_{k}^{\dom(\gamma)}])_{ij}$. 
  Hence, by projecting in attributes $\lbrace \row_\alpha, \col_\beta\rbrace$ we range over all $k$ and sum up all $K$-values for each entry.
\end{itemize}

Here, we only allow $\kprod$ function application. 
Note that we can access the zero values of matrices because the indexes are in the active domain of $\text{Rel}(\I)$ due to the existence of $R_\alpha^{\text{Rel}(\I)}(t)$, for each $\alpha \in \DD$.
\qed

% Consider a matrix instance $\I = (\dom,\conc)$ over a schema $\Sch$.
% Let $V\in\Mnam$ with $\size(V)=(\alpha,\beta)$ and let $\conc(V)$ be its corresponding matrix of dimension $\dom(\alpha)\times \dom(\beta)$.
% Given an instance $\I$ over $\Sch$, the domain asssignment $\mathbb{D}_{\I}$ is defined as 
% $\mathbb{D}_{\I}(\row_\alpha)=[1,\dom(\alpha)]$ and 
% $\mathbb{D}_{\I}(\col_\alpha)=[1,\dom(\alpha)]$. 
% We further  define the database instance $\text{Rel}_\Sch(\I)$  to consist of relations for each $V_R\in N$ defined as follows:
% $\mathcal{T}_{\mathbb{D}_{\I}}(\text{Rel}(\Sch)(V_R)) \to K$ such that
% $(\text{Rel}_{_\Sch}(I))(t):=\conc(V)_{ij}$ where (1) $t(\row_\alpha)=i$ if $\alpha\neq 1$ and equal to $1$ if $\alpha = 1$; and (2) $t(\col_\beta)=j$ if $\beta\neq 1$ and equal to $1$ if $\beta= 1$.

% We next translate \lang$(\sum,\prod)$ expressions $e$ into \ARA expressions $\Phi(e)$ by induction on the structure of $e$. The translation closely follows the translation given in~\cite{brijder2019matrices}, except that we  additionally need to consider summation, pointwise functions and the $\star$-projection.

% \begin{itemize}
% 	\item If $e=V$ then $\Phi(e):=V_R$.
% 	\item if $e=e_1^t$ where $\Sch(e_1)=(\alpha,\beta)$ then \[
% \Phi(e) :=
% \begin{cases}
% \rho_{\mathrm{col}_\alpha \to \mathrm{row}_\alpha,\mathrm{row}_\beta \to \mathrm{col}_\beta}\bigl(\Phi(e_1)\bigr) & \text{if } \alpha \neq 1 \neq \beta; \cr
% \rho_{\mathrm{col}_\alpha \to \mathrm{row}_\alpha}\bigl(\Phi(e_1)\bigr) & \text{if } \alpha \neq 1 = \beta; \cr
% \rho_{\mathrm{row}_\beta \to \mathrm{col}_\beta}\bigl(\Phi(e_1)\bigr) & \text{if } \alpha = 1 \neq \beta; \cr
% \Phi(e_1) & \text{if } \alpha = 1 = \beta,
% \end{cases}
% \]

% \item
% 	If $e = e_1 \cdot e_2$ where $\Sch(e_1) = (\alpha,\gamma)$ and $\Sch(e_2) =(\gamma,\beta)$, then we consider two cases. If $\gamma = 1$, then $\Phi(e) := \Phi(e_1) \Join \Phi(e_2)$. If $\gamma \neq 1$, then 
% 	$$
% 	\Phi(e) := \hat{\pi}_C\Bigr(\rho_{\mathrm{col}_\gamma\to C}\bigl(\Phi(e_1)\bigr)\Join\rho_{\mathrm{row}_\gamma\to C}\bigl(\Phi(e_2)\bigr)\Bigr).$$
% 	% , where $\varphi_1(\mathrm{col}_\gamma) = \varphi_2(\mathrm{row}_\gamma) = C \notin \{\mathrm{row}_\alpha, \mathrm{col}_\beta\}$ and $\varphi_1$ and $\varphi_2$ are the identity otherwise.
% 	% If $e=e_1(v_1,\ldots,v_k)\cdot e_2(u_1,\ldots,u_s)$ where $e_1$ is $n\times\gamma$, $e_2$ is $\gamma\times m$. Let $\rho:\row_\gamma\rightarrow C,\col_\gamma\rightarrow C.$ We have two cases:
% 	% 	\begin{itemize}
% 	% 		\item If $\gamma\neq 1$ then $E=\widehat{\pi}_C\left( \rho\left(E_1\right)\bowtie\rho\left( E_2\right)\right).$
% 	% 		\item If $\gamma = 1$ then $E=E_1\bowtie E_2$.
% 	% 	\end{itemize}
% 	\item If $e=f(e_1,\ldots,e_k)$ with $\Sch(e_i)=(1,1)$ for all $i\in[1,k]$, then
% 	$\Phi(e):=\text{Apply}[f]\bigl(\Phi(e_1),\ldots,\Phi(e_k)\bigr)$. 
% 	% we have that $E=E_1\cup\cdots\cup E_s$ if $f$ is sum and $E=E_1\bowtie\cdots\bowtie E_s$ if $f$ is multiplication.
% 	\item If $e=\ssum V.e_1$ where $\Sch(e_1)=(\alpha,\beta)$ and $\Sch(V)=(\gamma,1)$. Then,
% 	in $\Phi(e_1)$ we replace $V_R$ by $\Phi_{Id}(V_R)$ which computes a binary 
% 	relation encoding the $\gamma\times\gamma$ idenity matrix. Intuitively, by selecting different
% 	columns of the identity matrix we can extract all canonical $\gamma\times 1$ basis vectors.
% 	More precisely, $\Phi_{Id}(V_R)$ is  defined by
% 	$$
% 	\sigma_{\{\mathrm{row}_\gamma,C_V\}}\Bigr(\mathbf{1}(V_R) \Join \mathbf{1}\bigl(\rho_{\mathrm{row}_\gamma \to C_V}(V_R)\bigr)\Bigr)$$
% 	if $\gamma \neq 1$ and
%    $\mathbf{1}(V_R)$ if $\gamma = 1$.
%    Then,
% 	$$
% 	\Phi(e):=\hat{\pi}_{C_V}\bigl(\Phi(e_1)[V_R\gets \Phi_{Id}(V_R)])\bigr).
% 	$$

% 	Note that when the $C_{V}$ attribute in $\Phi(e_1[V_R\gets \Phi_{Id}(V_R)])$
% 	is instantiated with a value $j$ in $[1,n_\gamma]$, then this expression evaluates $e_1(\I[V\gets e_j^\gamma])$
% 	Hence, by projecting over $C_V$ we range over all $j\in[1,n_\gamma]$ and sum up all $K$-values for each entry. 
% \end{itemize}

% \begin{proposition}
% 	For each \lang$(\sum,\prod)$ expression $e$ over schema $\Sch$ such that $\Sch(e)=(\alpha,\beta)$ with $\alpha\neq 1\neq\beta$, there exists an \ARA expression $\Phi(e)$ over schema $\text{Rel}(\Sch)$ such that $\text{Rel}(\Sch)(\Phi(e))=\{\mathrm{row}_\alpha,\mathrm{col}_\beta\}$ and 
% 	such that for any instance $\I$ over $\Sch$,
% 	$$
% 	e(\I)_{i,j}=\Phi(e)(\text{Rel}_{\Sch}(\I))(t)
% 	$$
% 	for tuple $t(\mathrm{row}_\alpha)=i$ and $t(\mathrm{col}_\beta)=j$ in $\text{Rel}_{\Sch}(\I)$. Similarly for when $e$ has schema $\Sch(e)=(\alpha,1)$, $\Sch(e)=(1,\beta)$ or $\Sch(e)=(1,1)$, then $\Phi(e)$ has schema $\text{Rel}(\Sch)(\Phi(e))=\{\mathrm{row}_\alpha\}$,
% $\text{Rel}(\Sch)(\Phi(e))=\{\mathrm{col}_\alpha\}$, or
% $\text{Rel}(\Sch)(\Phi(e))=\{\}$, respectively.
% \end{proposition}

% For the converse translation, i.e., from \ARA to \lang++, we need to impose some restrictions. More precisely, we only consider \ARA expression $\varphi$
% that take as input relations of arity at most two and also have a schema of arity at most two. Note that intermediate expressions can create schemas of arbitraty size. We also make the assumption that there is an order, denoted by $<$, on the attributes in $\mathbf{att}$. In particular, we assume $A_1<A_2<\cdots$ for attributes $A_i\in\mathbf{att}$.

% This is to identify which attributes correspond to rows and columns when moving the matrix setting. 


% Consider a database schema $\mathcal{R}$ on a finite set $N$ of relation names
%  assigning a relation schema $\mathcal{R}(R)\subseteq\mathbf{att}$ to each $R \in N$. We assume that $\mathcal{R}(R)$ has size at most two. With each relation name $R\in N$ we associate a matrix name $M_R$. Let $\text{Mat}(\mathcal{R})$ denote the set
%  $V_R$ of matrix names for $R\in\mathcal{R}$. Consider an injective function $s:\mathbf{att}\to \DD$ associating with each attribute a unique size symbol. Let $V_R\in \text{Mat}(\mathcal{R})$ and
% define
%  $$
% \size(V_R)=\begin{cases}
% (s(A_1),s(A_2)) & \text{if $\mathcal{R}(R)=\{A_1,A_2\}$, $A_1<A_2$}\\
% (s(A),1) & \text{if $\mathcal{R}(R)=\{A\}$}\\
% (1,1) & \text{if $\mathcal{R}(R)=\{\}$}.
% \end{cases}
%  $$
% Let $\mathbb{D}$ be a domain assignment. We define 
% $\dom(\alpha)=|\mathbb{D}(A)|$ where $s(A)=\alpha$.
% We only consider consecutive domain assignments, i.e.,
% such that attribute values take values in $[1,||\mathbb{D}(A)|]$.
% Consider 
% a relation $r:
% \mathcal{T}_{\mathbb{D}}(X) \to K$ of $R$ with $X\subseteq\{A_1,A_2\}$  as determined by
% $\mathcal{R}(R)$. We associate a matrix instance $\I = (\dom,\conc)$ as follows.
% We define $\dom(\alpha)=|\mathbb{D}(A_1)|$ and
% $\dom(\beta)=|\mathbb{D}(A_2)|$ where $s(A_1)=\alpha$ and $s(A_2)=\beta$. Furthermore,
% $\conc(V_R)=\text{Mat}(r)$ such that 
% $(\text{Mat}(r))_{i,j} := r(t)$, where $t$ is (1) the tuple with $t(A_1) = i$ and $t(A_2) = j$ if $|X| = 2$; (2) the tuple with $t(A_1) = i$ and $j = 1$ if $X = {A_1}$,
% (3) the tuple with $t(A_2) = j$ and $i = 1$ if $X = {A_2}$,
% (3) the unique tuple of $r$ if $X=\emptyset$. Clearly, $\text{Mat}(r)$ is a matrix of dimension as
% specified by $\mathbb{D}$. 


% %
% % In the following, when $\varphi$ is
% % an \ARA expression of schema $\mathcal{R}(\varphi)=\{A_1,\ldots,A_k\}$ with $A_1<A_2<A_3<\cdots < A_k$
% %
% We next translate \ARA expressions in to \lang$(\sum,\prod)$ expressions over an extended schema. More specifically, we extend 
% $\Mnam$ with matrix variables $V_A$ for attributes $A$ appearing the \ARA expression. We first simulate \ARA expression entry-wise.

% \begin{lemma}
% For every \ARA expression $\varphi$ over schema $\mathcal{R}$ with there is \lang$(\sum,\prod)$ expression $\Upsilon(\varphi)$ such that for every database instances $\I$ over $\mathcal{R}$ using consecutive domain assignment, 
% $$
% \varphi(\I)(i_1,\ldots,i_p)=\Upsilon(\varphi)(\text{Mat}(\I)\cup \{e_{i_1}^{n_1},\ldots,e_{i_p}^{n_p})
% $$
% \end{lemma}
% \begin{proof}
% \begin{itemize}
% \item If $\varphi=R$, then $\Upsilon(e):=V_{A_1}^t\cdot V_R\cdot V_{A_2}$ if $\mathcal{R}(R)=\{A_1,A_2\}$ with $A_1<A_2$; 
% $\Upsilon(e):=V_A^t\cdot V_R$ if $\mathcal{R}(R)=\{A\}$; and 
% $\Upsilon(e):=V_R$ if $\mathcal{R}(R)=\{\}$. We define $\text{Ext}()$
% \item If $\varphi=\mathbf{1}(\psi)$  then $
% \Upsilon(\varphi):=\text{Apply}[x\mapsto 1](\Upsilon(\psi))$.
% \item If $\varphi=\psi_1\cup \psi_2$ then
% $\Upsilon(\varphi):=\text{Apply}[(x,y)\mapsto x+y](\Upsilon(\psi_1),\Upsilon(\psi_2))$.
% \item If $\varphi=\pi_{Y}(\psi)$ for $Y\subseteq \mathcal{R}(\psi)$ then
% $$
% \Upsilon(\varphi):=\sum_{\{V_A\mid A\in \mathcal{R}(\psi)\setminus Y\}}\Upsilon(\psi).
%  $$
% \item If $\varphi=\sigma_{Y}(\psi)$ with $Y\subseteq\mathcal{R}(\psi)$ then
% $$
%  \Upsilon(\varphi):=\Upsilon(\psi)\cdot\prod_{A,B\in Y} V_{A}^t\cdot V_{B}.
% $$
% \item If $\varphi=\rho_{X\mapsto Y}(\psi)$ then
% $$\Upsilon(\varphi):=\Upsilon(\psi)[V_A\gets V_B\mid A\in X, B\in Y, A\mapsto B].$$
% \item If $\varphi=\psi_1\bowtie \psi_2$ then
% $\Upsilon(\varphi):=\Upsilon(\psi_1)\cdot \Upsilon(\psi_2)$.
% \item If $\varphi=\pi_{Y}^\star(\psi)$ for $Y\subseteq \mathcal{R}(\psi)$.
% \item If $\varphi=\text{Apply}[f](\psi_1,\ldots,\psi_k)$  then
% $\Upsilon(\varphi):=\text{Apply}[f](\Upsilon(\psi_1),\ldots,\Upsilon(Y_k))$.
% \end{itemize}
% \end{proof}
% As a consequence, when $\varphi$ is an \ARA expression such that $\mathcal{R}(\varphi)=\{A_1,A_2\}$ with $A_1<A_2$ we have that 
% $$
% \varphi(\I)(t)=
% \sum_{V_{A_1},V_{A_2}}\Upsilon(\varphi)\cdot V_{A_1}\cdot V_{A_2}^t.
% $$
% When $\mathcal{R}(\varphi)=\{A\}$ we have
% $$
% \varphi(\I)(t)=
% \sum_{V_{A}}\Upsilon(\varphi)\cdot V_{A_1}.
% $$
% and
% when $\mathcal{R}(\varphi)=\{\}$ we have
% $$
% \varphi(\I)(t)=\Upsilon(\varphi).
% $$
 


